Progress on supercompilation

theories/Transform/ReadOffPreproof.v
@@ -3,39 +3,77 @@ From stdpp Require Import prelude countable gmap.
 
 From Cyclic.Graph Require Import FiniteDigraph.
 From Cyclic.Preproof Require Import Preproof.
-From Cyclic.Transform Require Import ReadOff.
+From Cyclic.Transform Require Import ReadOff CyclicRules.
 
 Import ListNotations.
 
 Set Default Proof Using "Type".
 
 Module RO := ReadOff.
+Module CR := CyclicRules.
 
 Section Packaging.
-  (** Package the raw read-off graph as a rooted preproof.
+  (** Package the raw read-off graph as a rooted preproof whose labels are
+      vertex-based judgements.
 
-      For now, the local rule is trivial (`True`). This step exists to move from
-      “maps representing a cyclic graph” to the project’s standard `preproof`
-      structure.
+      This is an incremental correctness step:
+      - substitution evidence nodes (`nSubstNil`/`nSubstCons`) are labelled by
+        `jSub` judgements and checked by the structural `jSub` rule.
+      - all other nodes are labelled by a dummy `jTy` judgement and are accepted
+        by a permissive rule (`True`) for now.
 
-      Next step: replace `Rule` by the vertex-typing/equality/substitution rule
-      relation (`jTyV/jEqV/jSubV`) and prove `pp_rule_ok` by construction.
+      Next step: strengthen `jTy`/`jEq` cases and make `pp_label` produce real
+      typing/equality goals.
   *)
 
-  Definition Judgement : Type := RO.node.
-  Definition Rule (_ : Judgement) (_ : list Judgement) : Prop := True.
+  Definition V : Type := nat.
 
-  Definition verts_of (b : RO.builder) : gset nat :=
+  Definition verts_of (b : RO.builder) : gset V :=
     dom (RO.b_label b).
 
-  Definition succ_of (b : RO.builder) (v : nat) : list nat :=
+  Definition succ_of (b : RO.builder) (v : V) : list V :=
     filter (fun w => bool_decide (w ∈ verts_of b))
       (default [] (RO.b_succ b !! v)).
 
-  Definition label_of (b : RO.builder) (v : nat) : RO.node :=
+  Definition label_of (b : RO.builder) (v : V) : RO.node :=
     default (RO.nVar 0) (RO.b_label b !! v).
 
-  Lemma succ_of_closed (b : RO.builder) (v : nat) :
+  Definition dummy_type : V := 0.
+
+  Fixpoint sub_ctx (fuel : nat) (b : RO.builder) (sv : V) : list V :=
+    match fuel with
+    | 0 => []
+    | S fuel' =>
+        match RO.b_label b !! sv with
+        | Some (RO.nSubstNil _) => []
+        | Some (RO.nSubstCons _) =>
+            match RO.b_succ b !! sv with
+            | Some [u; sv_tail] => dummy_type :: sub_ctx fuel' b sv_tail
+            | _ => []
+            end
+        | _ => []
+        end
+    end.
+
+  Definition shiftV (_n _k : nat) (x : V) : V := x.
+  Definition substV (_sv : V) (x : V) : V := x.
+
+  Definition Judgement : Type := CR.judgement (V := V).
+
+  Definition pp_label (b : RO.builder) (v : V) : Judgement :=
+    match label_of b v with
+    | RO.nSubstNil _ => CR.jSub (V := V) [] v (sub_ctx (RO.b_next b + 1) b v)
+    | RO.nSubstCons _ => CR.jSub (V := V) [] v (sub_ctx (RO.b_next b + 1) b v)
+    | _ => CR.jTy (V := V) [] v dummy_type
+    end.
+
+  Definition Rule (b : RO.builder) (j : Judgement) (premises : list Judgement) : Prop :=
+    match j with
+    | CR.jSub _ _ _ => CR.rule (V := V) (label_of b) (succ_of b) shiftV substV j premises
+    | _ => True
+    end.
+
+  Lemma succ_of_closed (b : RO.builder) (v : V) :
     Forall (fun w => w ∈ verts_of b) (succ_of b v).
   Proof.
     apply Forall_forall.
@@ -46,7 +84,7 @@ Section Packaging.
     now apply bool_decide_true in Hw.
   Qed.
 
-  Program Definition graph_of (b : RO.builder) : FiniteDigraph.fin_digraph nat :=
+  Program Definition graph_of (b : RO.builder) : FiniteDigraph.fin_digraph V :=
     {| FiniteDigraph.verts := verts_of b;
        FiniteDigraph.succ := succ_of b |}.
   Next Obligation.
@@ -54,10 +92,26 @@ Section Packaging.
     exact (succ_of_closed b v).
   Qed.
 
-  Definition preproof_of (b : RO.builder) : @Preproof.preproof Judgement Rule nat _ _ :=
+  Lemma pp_rule_ok (b : RO.builder) (v : V) :
+    v ∈ verts (graph_of b) ->
+    Rule b (pp_label b v) (map (pp_label b) (succ (graph_of b) v)).
+  Proof.
+    intro Hv.
+    unfold Rule.
+    unfold pp_label.
+    destruct (label_of b v) eqn:Hlbl; simpl; try exact I.
+    all: (* substitution vertices *)
+      unfold CR.rule; simpl.
+      (* The `jSub` rule is a definitional match; our premises are the labels of
+         successor vertices, so this closes by computation. *)
+      tauto.
+  Qed.
+
+  Definition preproof_of (b : RO.builder)
+      : @Preproof.preproof Judgement (Rule b) V _ _ :=
     {| Preproof.pp_graph := graph_of b;
-       Preproof.pp_label := label_of b;
-       Preproof.pp_rule_ok := fun _ _ => I |}.
+       Preproof.pp_label := pp_label b;
+       Preproof.pp_rule_ok := fun v Hv => pp_rule_ok b v Hv |}.
 
   Lemma compile_tm_root_label (fuel : nat) (ρ : RO.back_env) (t : Term.Syntax.tm)
       (b : RO.builder) (root : nat) (b' : RO.builder) :
@@ -67,44 +121,19 @@ Section Packaging.
     revert ρ t b root b'.
     induction fuel as [|fuel IH]; intros ρ t b root b' H;
       simpl in H.
-    - (* fuel = 0 *)
-      destruct (RO.fresh b) as [v0 b0] eqn:Hfresh.
+    - destruct (RO.fresh b) as [v0 b0] eqn:Hfresh.
       inversion H; subst.
       unfold RO.put.
       simpl.
       rewrite lookup_insert.
-      eexists.
-      reflexivity.
-    - (* fuel = S fuel *)
-      destruct t; try (destruct (RO.fresh b) as [v0 b0] eqn:Hfresh; inversion H; subst;
+      eexists; reflexivity.
+    - destruct t; simpl in H.
+      all: try (destruct (RO.fresh b) as [v0 b0] eqn:Hfresh; inversion H; subst;
         unfold RO.put; simpl; rewrite lookup_insert; eexists; reflexivity).
-      all: try (destruct (RO.fresh b) as [v0 b0] eqn:Hfresh;
-        (* the remaining cases perform recursive compilation but always end by `put v0 ...` *)
+      (* Remaining constructors call `put` at the returned root. *)
+      all: try (repeat (destruct (RO.fresh b) as [v0 b0] eqn:Hfresh); clear Hfresh;
         repeat (destruct (RO.compile_tm fuel _ _ _ ) as [vx bx] eqn:?);
         inversion H; subst; unfold RO.put; simpl; rewrite lookup_insert; eexists; reflexivity).
-      (* tApp case *)
-      + (* tApp *)
-        destruct (RO.app_view (Term.Syntax.tApp t1 t2)) as [h args] eqn:Hview.
-        destruct h.
-        * (* head is a variable *)
-          destruct (nth_error ρ x) as [[target|]|] eqn:Hnth.
-          -- (* backlink case *)
-             (* after allocating the backlink vertex we always `put` it *)
-             repeat (destruct (RO.compile_tm fuel ρ _ _) as [vx bx] eqn:?);
-             repeat (destruct (RO.fresh _) as [vx bx] eqn:?);
-             inversion H; subst; unfold RO.put; simpl; rewrite lookup_insert; eexists; reflexivity.
-          -- (* non-backlink *)
-             destruct (RO.fresh b) as [v0 b0] eqn:Hfresh.
-             repeat (destruct (RO.compile_tm fuel _ _ _ ) as [vx bx] eqn:?);
-             inversion H; subst; unfold RO.put; simpl; rewrite lookup_insert; eexists; reflexivity.
-          -- (* non-backlink *)
-             destruct (RO.fresh b) as [v0 b0] eqn:Hfresh.
-             repeat (destruct (RO.compile_tm fuel _ _ _ ) as [vx bx] eqn:?);
-             inversion H; subst; unfold RO.put; simpl; rewrite lookup_insert; eexists; reflexivity.
-        * (* head is not a variable *)
-          destruct (RO.fresh b) as [v0 b0] eqn:Hfresh.
-          repeat (destruct (RO.compile_tm fuel _ _ _ ) as [vx bx] eqn:?);
-          inversion H; subst; unfold RO.put; simpl; rewrite lookup_insert; eexists; reflexivity.
   Qed.
 
   Lemma read_off_root_in (t : Term.Syntax.tm) (root : nat) (b : RO.builder) :
@@ -120,7 +149,7 @@ Section Packaging.
   Qed.
 
   Definition rooted_preproof_of (t : Term.Syntax.tm)
-      : @Preproof.rooted_preproof Judgement Rule nat _ _ :=
+      : @Preproof.rooted_preproof Judgement (fun j ps => Rule (snd (RO.read_off_raw t)) j ps) V _ _ :=
     let '(root, b) := RO.read_off_raw t in
     {| Preproof.rpp_proof := preproof_of b;
        Preproof.rpp_root := root;
